with Aymeric and Denis, a two-phase tactic for frame_delta (still with an admit)

pulse/ulib/LowStar.RST.Tactics.fst
@@ -45,16 +45,95 @@ inline_for_extraction noextract let rm : cm resource req =
      equal_comm_monoid_commutativity
      equal_comm_monoid_cong
 
-inline_for_extraction noextract let resolve_delta (outer inner:term) : Tac unit =
-  norm [delta_only [`%frame_delta]];
-  refine_intro ();
-  flip ();
+
+inline_for_extraction noextract let resolve_frame_delta' () : Tac unit =
   split ();
+  dump "4";      
   norm [delta_only [`%frame_delta_pre]];
+  dump "5";        
   apply_lemma (quote can_be_split_into_star);
+  dump "6";          
   flip ();
+  dump "7";          
   canon_monoid req rm;
+  dump "8";            
   norm [delta_only [`%frame_delta_post]];
+  dump "9";              
   ignore (forall_intro ());
+  dump "10";              
   apply_lemma (quote can_be_split_into_star);
-  canon_monoid req rm
+  dump "11";                
+  canon_monoid req rm;
+  dump "12"
+
+let squash_and p q (x:squash (p /\ q)) : (p /\ q) = 
+  let x : squash (p `c_and` q) = FStar.Squash.join_squash x in
+  x
+
+inline_for_extraction noextract let resolve_frame_delta () : Tac unit =
+  dump "Second phase: 1";
+  norm [delta_only [`%frame_delta]];
+  dump "Second phase: 2";  
+  apply (`squash_and);
+  resolve_frame_delta' ()
+
+let unfold_with_tactic (t:unit -> Tac 'a) (p:Type)
+  : Lemma (requires p)
+          (ensures (with_tactic t p))
+  = admit()
+
+
+let foobar () : Tac unit = 
+  dump "A";
+  refine_intro ();
+  dump "B";  
+  flip ();
+  dump "C";    
+  apply_lemma (`unfold_with_tactic);
+  dump "D";    
+  exact (`0)
+
+let l_True_term : l_True = ()
+
+let baz () : Tac unit = 
+  dump "Z";
+  exact (`l_True_term)
+
+assume val test (#[foobar()] x : int { FStar.Tactics.with_tactic baz True }) (y:bool) : unit
+
+let atest (p q: Type) =
+  let x : (p /\ q) = _ by (apply (`squash_and); dump "A"; tadmit()) in
+  ()
+
+let run () = 
+    test true
+
+inline_for_extraction noextract let resolve_delta () : Tac unit =
+  dump "1";
+  refine_intro ();
+  dump "2";  
+  flip ();
+  dump "3";  
+  apply_lemma (`unfold_with_tactic);
+  dump "3.1";  
+  norm [delta_only [`%frame_delta]];
+  dump "3.2";  
+  resolve_frame_delta' ()
+  // split ();
+  // dump "4";      
+  // norm [delta_only [`%frame_delta_pre]];
+  // dump "5";        
+  // apply_lemma (quote can_be_split_into_star);
+  // dump "6";          
+  // flip ();
+  // dump "7";          
+  // canon_monoid req rm;
+  // dump "8";            
+  // norm [delta_only [`%frame_delta_post]];
+  // dump "9";              
+  // ignore (forall_intro ());
+  // dump "10";              
+  // apply_lemma (quote can_be_split_into_star);
+  // dump "11";                
+  // canon_monoid req rm;
+  // dump "12"
